---
layout: post
title: "Humam Fauzi Math First Post"
date: 2015-04-30
category: Math
tags: ["TeX"]
---

$$k_{\,1,i} = f(t_{1,n}+c_ih, t_{2,n}+c_ih, \cdots , t_{n,n}+c_ih \quad ; \quad y_{1,n} +h\sum_{j=1}^{i-1}a_{i-1,\,j}k_{\, 1,i-1},\; y_{2,n} +h\sum_{j=1}^{i-1}a_{i-1,\,j}k_{\, 2,i-1}, \cdots ,y_{n,n} +h\sum_{j=1}^{i-1}a_{i-1,\,j}k_{\, n,i-1})$$
$$k_{\,2,i} = f(t_{1,n}+c_ih, t_{2,n}+c_ih, \cdots , t_{n,n}+c_ih \quad ; \quad y_{1,n} +h\sum_{j=1}^{i-1}a_{i-1,\,j}k_{\, 1,i-1},\; y_{2,n} +h\sum_{j=1}^{i-1}a_{i-1,\,j}k_{\, 2,i-1}, \cdots ,y_{n,n} +h\sum_{j=1}^{i-1}a_{i-1,\,j}k_{\, n,i-1})$$
$$k_{\,3,i} = f(t_{1,n}+c_ih, t_{2,n}+c_ih, \cdots , t_{n,n}+c_ih \quad ; \quad y_{1,n} +h\sum_{j=1}^{i-1}a_{i-1,\,j}k_{\, 1,i-1},\; y_{2,n} +h\sum_{j=1}^{i-1}a_{i-1,\,j}k_{\, 2,i-1}, \cdots ,y_{n,n} +h\sum_{j=1}^{i-1}a_{i-1,\,j}k_{\, n,i-1})$$
$$\vdots$$
$$k_{\,n,i} = f(t_{1,n}+c_ih, t_{2,n}+c_ih, \cdots , t_{n,n}+c_ih \quad ; \quad y_{1,n} +h\sum_{j=1}^{i-1}a_{i-1,\,j}k_{\, 1,i-1},\; y_{2,n} +h\sum_{j=1}^{i-1}a_{i-1,\,j}k_{\, 2,i-1}, \cdots ,y_{n,n} +h\sum_{j=1}^{i-1}a_{i-1,\,j}k_{\, n,i-1})$$

